coq/theories/automation/Automation.v
@@ -1,0 +1,20 @@
+Require Import impboot.functional.FunValues.
+Require Import impboot.functional.FunSyntax.
+Require Import impboot.functional.FunSemantics.
+Require Import impboot.automation.AutomationLemmas.
+Require Import impboot.utils.Llist.
+Require Import Coq.Bool.Bool.
+Require Import Coq.Lists.List.
+Import ListNotations.
+Require Import Lia Nat Arith.
+
+Definition empty_state : state := init_state lnil [].
+
+
+(* TODO(kπ) figure out a good example, this one gets constant folded *)
+Example arith_example : forall n m,
+  exists prog, Env.empty |- (prog, empty_state) ---> ([Num (let x := 1 in x + n - m)], empty_state).
+Proof.
+  intros.
+  eauto with automation.
+Qed.
