coq/theories/automation/AutomationLemmas.v
@@ -1,0 +1,248 @@
+Require Import impboot.functional.FunSyntax.
+Require Import impboot.functional.FunSemantics.
+Require Import impboot.functional.FunProperties.
+Require Import impboot.functional.FunValues.
+Require Import Coq.Lists.List.
+Import ListNotations.
+Require Import Lia Nat Arith.
+
+Create HintDb automation.
+
+Theorem trans_app: forall n params vs b body s s1 v,
+  let env := make_env params vs Env.empty in
+    (b -> (env |- ([body], s) ---> ([v], s1))) ->
+    List.length params = List.length vs ->
+    lookup_fun (value_name n) s.(funs) = Some (params,body) ->
+    b -> eval_app (value_name n) vs s (v,s1).
+Proof.
+  intros; eapply App_intro; eauto.
+  unfold env_and_body; simpl.
+  rewrite H1.
+  rewrite <- Nat.eqb_eq in H0; rewrite H0.
+  reflexivity.
+Qed.
+
+Theorem trans_Call : forall b1 b2 env xs s1 s2 s3 fname vs v,
+  (b1 -> env |- (xs, s1) ---> (vs, s2)) ->
+  (b2 -> eval_app fname vs s2 (v, s3)) ->
+  (b1 /\ b2 -> env |- ([Call fname xs], s1) ---> ([v], s3)).
+Proof.
+  intros b1 b2 env xs s1 s2 s3 fname vs v H1 H2 [Hb1 Hb2].
+  apply H1 in Hb1; apply H2 in Hb2.
+  inversion Hb2; subst.
+  eapply Eval_Call with (vs := vs) (s2 := s2); eauto.
+Qed.
+
+Theorem trans_Var : forall n v env s,
+  Env.lookup env (value_name n) = Some v ->
+  env |- ([Var (value_name n)], s) ---> ([v], s).
+Proof.
+  intros n v env s H.
+  apply Eval_Var; auto.
+Qed.
+
+Theorem trans_nil : forall env s,
+  env |- ([], s) ---> ([], s).
+Proof.
+  intros env s.
+  apply Eval_Nil.
+Qed.
+
+Theorem trans_cons : forall x xs v vs env s s1 s2,
+  env |- ([x], s) ---> ([v], s1) ->
+  env |- (xs, s1) ---> (vs, s2) ->
+  env |- (x :: xs, s) ---> (v :: vs, s2).
+Proof.
+  intros x xs v vs env s s1 s2 H1 H2.
+  destruct xs; simpl in *.
+  - inversion H2; subst.
+    assumption.
+  - inversion H2; subst; econstructor; eauto.
+Qed.
+
+Theorem auto_let : forall {A : Type} {B : Type}
+    b1 b2 (a : A -> Value) (b : B -> Value) env x1 y1 s1 s2 s3 v1 let_n f,
+  (b1 -> env |- ([x1], s1) ---> ([a v1], s2)) ->
+  (forall v1, b2 v1 -> (Env.insert ((value_name let_n), a v1) env) |- ([y1], s2) ---> ([b (f v1)], s3)) ->
+  (b1 /\ b2 v1 ->
+    env |- ([Let (value_name let_n) x1 y1], s1) ---> ([b (f v1)], s3)).
+Proof.
+  intros.
+  destruct H1.
+  eapply Eval_Let; eauto.
+Qed.
+
+Theorem auto_otherwise : forall {A : Type}
+    b1 (a : A -> Value) env s x1 v1,
+  (b1 -> env |- ([x1], s) ---> ([a v1], s)) ->
+  (b1 ->
+    env |- ([If Less [Const 0; Const 1] x1 (Const 0)], s) ---> ([a (value_otherwise v1)], s)).
+Proof.
+  intros.
+  apply H in X.
+  repeat econstructor; eauto.
+Qed.
+
+(* bool *)
+
+Theorem auto_bool_F : forall env s,
+  env |- ([Const 0], s) ---> ([value_bool false], s).
+Proof.
+  intros. apply Eval_Const.
+Qed.
+Hint Resolve auto_bool_F : automation.
+
+Theorem auto_bool_T : forall env s,
+  env |- ([Const 1], s) ---> ([value_bool true], s).
+Proof.
+  intros. apply Eval_Const.
+Qed.
+Hint Resolve auto_bool_T : automation.
+
+Ltac Eval_eq :=
+  repeat match goal with
+  | _ => progress simpl in *
+  | _ => lia
+  | _ => congruence
+  | _ => econstructor
+  | _ => eauto
+  end.
+
+Theorem auto_bool_not : forall env s x1 b,
+  env |- ([x1], s) ---> ([value_bool b], s) ->
+  env |- ([Op Sub [Const 1; x1]], s) ---> ([value_bool (negb b)], s).
+Proof.
+  intros env s x1 b H.
+  Eval_eq.
+  destruct b; simpl; eauto with automation.
+Qed.
+Hint Resolve auto_bool_not : automation.
+
+Theorem auto_bool_and : forall env s x1 x2 bA bB,
+  env |- ([x1], s) ---> ([value_bool bA], s) ->
+  env |- ([x2], s) ---> ([value_bool bB], s) ->
+  env |- ([Op Sub [Op FunSyntax.Add [x1; x2]; Const 1]], s) ---> ([value_bool (andb bA bB)], s).
+Proof.
+  intros env s x1 x2 bA bB H1 H2.
+  destruct (value_bool bA) eqn:HbA; destruct (value_bool bB) eqn:HbB; simpl in *.
+  all: unfold value_bool in *; simpl in *; destruct bA; destruct bB; inversion HbA; inversion HbB; subst.
+  all: Eval_eq.
+Qed.
+Hint Resolve auto_bool_and : automation.
+
+Theorem auto_bool_iff : forall env s x1 x2 bA bB,
+  env |- ([x1], s) ---> ([value_bool bA], s) ->
+  env |- ([x2], s) ---> ([value_bool bB], s) ->
+  env |- ([If Equal [x1; x2] (Const 1) (Const 0)], s) ---> ([value_bool (Bool.eqb bA bB)], s).
+Proof.
+  intros env s x1 x2 bA bB H1 H2.
+  destruct (value_bool bA) eqn:HbA; destruct (value_bool bB) eqn:HbB; simpl in *.
+  all: unfold value_bool in *; simpl in *; destruct bA; destruct bB; inversion HbA; inversion HbB; subst.
+  all: Eval_eq.
+Qed.
+Hint Resolve auto_bool_iff : automation.
+
+Theorem last_bool_if : forall env s x_g x_t x_f b t f,
+  env |- ([x_g], s) ---> ([value_bool b], s) ->
+  env |- ([x_t], s) ---> ([t], s) ->
+  env |- ([x_f], s) ---> ([f], s) ->
+  env |- ([If Equal [x_g; Const 1] x_t x_f], s) ---> ([if b then t else f], s).
+Proof.
+  intros env s x_g x_t x_f b t f H1 H2 H3.
+  destruct (value_bool b) eqn:Hb; simpl in *.
+  all: unfold value_bool in *; simpl in *; destruct b; inversion Hb; subst.
+  all: Eval_eq.
+Qed.
+Hint Resolve last_bool_if : automation.
+
+(* num *)
+
+Theorem auto_num_const_zero : forall env s,
+  env |- ([Const 0], s) ---> ([Num 0], s).
+Proof.
+  intros. apply Eval_Const.
+Qed.
+Hint Resolve auto_num_const_zero : automation.
+
+Theorem auto_num_const : forall env s n,
+  env |- ([Const n], s) ---> ([Num n], s).
+Proof.
+  intros. apply Eval_Const.
+Qed.
+Hint Resolve auto_num_const : automation.
+
+Theorem auto_num_add : forall b0 b1 env s0 s1 s2 x1 x2 n1 n2,
+  (b0 -> env |- ([x1], s0) ---> ([Num n1], s1)) ->
+  (b1 -> env |- ([x2], s1) ---> ([Num n2], s2)) ->
+  (b0 /\ b1 -> env |- ([Op FunSyntax.Add [x1; x2]], s0) ---> ([Num (n1 + n2)], s2)).
+Proof.
+  intros.
+  destruct H1.
+  repeat econstructor; eauto.
+Qed.
+
+Theorem auto_num_sub : forall b0 b1 env s0 s1 s2 x1 x2 n1 n2,
+  (b0 -> env |- ([x1], s0) ---> ([Num n1], s1)) ->
+  (b1 -> env |- ([x2], s1) ---> ([Num n2], s2)) ->
+  (b0 /\ b1 -> env |- ([Op FunSyntax.Sub [x1; x2]], s0) ---> ([Num (n1 - n2)], s2)).
+Proof.
+  intros.
+  destruct H1.
+  repeat econstructor; eauto.
+Qed.
+
+Theorem auto_num_div : forall b0 b1 env s0 s1 s2 x1 x2 n1 n2,
+  (b0 -> env |- ([x1], s0) ---> ([Num n1], s1)) ->
+  (b1 -> env |- ([x2], s1) ---> ([Num n2], s2)) ->
+  (b0 /\ b1 /\ n2 <> 0 -> env |- ([Op FunSyntax.Div [x1; x2]], s0) ---> ([Num (n1 / n2)], s2)).
+Proof.
+  intros.
+  destruct H1; destruct H2.
+  repeat econstructor; eauto.
+  rewrite <- Nat.eqb_neq in *; simpl; rewrite H3; unfold return_; reflexivity.
+Qed.
+
+Theorem auto_num_if_eq : forall {A : Type}
+    b0 b1 b2 b3 env s x1 x2 y z n1 n2 t f (a : A -> Value),
+  (b0 -> env |- ([x1], s) ---> ([Num n1], s)) ->
+  (b1 -> env |- ([x2], s) ---> ([Num n2], s)) ->
+  (b2 -> env |- ([y], s) ---> ([a t], s)) ->
+  (b3 -> env |- ([z], s) ---> ([a f], s)) ->
+  b0 /\ b1 /\ (if n1 =? n2 then b2 else b3) ->
+  env |- ([If Equal [x1; x2] y z], s) ---> ([a (if n1 =? n2 then t else f)], s).
+Proof.
+  intros.
+  destruct H3 as [Hb0 [Hb1 HbCond]].
+  apply H0 in Hb1.
+  apply H in Hb0.
+  destruct (n1 =? n2) eqn:Heq; [apply H1 in HbCond | apply H2 in HbCond].
+  all: repeat econstructor; eauto.
+  all: match goal with
+  | [ |- take_branch _ _ _ = _ ] => unfold take_branch, return_; reflexivity
+  | [ |- (_ |- (_, _) ---> (_, _)) ] => rewrite Heq; assumption
+  end.
+Qed.
+
+Theorem auto_num_if_less : forall {A : Type}
+    b0 b1 b2 b3 env s x1 x2 y z n1 n2 t f (a : A -> Value),
+  (b0 -> env |- ([x1], s) ---> ([Num n1], s)) ->
+  (b1 -> env |- ([x2], s) ---> ([Num n2], s)) ->
+  (b2 -> env |- ([y], s) ---> ([a t], s)) ->
+  (b3 -> env |- ([z], s) ---> ([a f], s)) ->
+  b0 /\ b1 /\ (if n1 <? n2 then b2 else b3) ->
+  env |- ([If Less [x1; x2] y z], s) ---> ([a (if n1 <? n2 then t else f)], s).
+Proof.
+  intros.
+  destruct H3 as [Hb0 [Hb1 HbCond]].
+  apply H0 in Hb1.
+  apply H in Hb0.
+  destruct (n1 <? n2) eqn:Heq; [apply H1 in HbCond | apply H2 in HbCond].
+  all: repeat econstructor; eauto.
+  all: match goal with
+  | [ |- take_branch _ _ _ = _ ] => unfold take_branch, return_; reflexivity
+  | [ |- (_ |- (_, _) ---> (_, _)) ] => rewrite Heq; assumption
+  end.
+Qed.
+
+(* TODO(kπ) continue *)
+
