coq/theories/functional/FunEnv.v
@@ -1,0 +1,72 @@
+Require Import Coq.Logic.FunctionalExtensionality.
+Require Import impboot.functional.FunValues.
+Require Import Arith Lia Nat.
+
+Module Type FunEnvT.
+  Parameter env : Type.
+  Parameter empty : env.
+  Parameter lookup : env -> name -> option Value.
+  Parameter insert : name * Value -> env -> env.
+  Parameter remove : name -> env -> env.
+
+  Axiom lookup_insert_eq : forall v x n,
+      lookup (insert (x, n) v) x = Some n.
+
+  Axiom lookup_insert_neq : forall v x1 x2 n,
+      x1 <> x2 ->
+      lookup (insert (x1, n) v) x2 = lookup v x2.
+
+  Axiom insert_insert_eq : forall v x n1 n2,
+      insert (x, n1) (insert (x, n2) v) = insert (x, n1) v.
+
+  Axiom insert_remove : forall v x n,
+      insert (x, n) (remove x v) = insert (x, n) v.
+
+  Axiom lookup_empty : forall x,
+      lookup empty x = None.
+
+End FunEnvT.
+
+Module FunEnv : FunEnvT.
+  Definition env := name -> option Value.
+  Definition empty : env := fun _ => None.
+  Definition lookup (v : env) (x : name) : option Value := v x.
+  Definition insert (p : name * Value) (v : env) : env :=
+    fun x => if x =? fst p then Some (snd p) else v x.
+  Definition remove (x : name) (v : env) : env :=
+    fun y => if x =? y then None else v y.
+
+  Theorem lookup_insert_eq : forall v x n,
+      lookup (insert (x, n) v) x = Some n.
+  Proof.
+    intros; unfold lookup, insert, fst; rewrite Nat.eqb_refl; reflexivity.
+  Qed.
+
+  Theorem lookup_insert_neq : forall v x1 x2 n,
+      x1 <> x2 ->
+      lookup (insert (x1, n) v) x2 = lookup v x2.
+  Proof.
+    intros; unfold lookup, insert, fst.
+    rewrite <- Nat.eqb_neq in H; rewrite Nat.eqb_sym in H; rewrite H.
+    reflexivity.
+  Qed.
+
+  Theorem insert_insert_eq : forall v x n1 n2,
+      insert (x, n1) (insert (x, n2) v) = insert (x, n1) v.
+  Proof.
+    intros; apply functional_extensionality; intros.
+    unfold insert; destruct (_ =? _); reflexivity.
+  Qed.
+
+  Theorem insert_remove : forall v x n,
+      insert (x, n) (remove x v) = insert (x, n) v.
+  Proof.
+    intros; apply functional_extensionality; intros.
+    unfold insert, remove, fst; destruct (_ =? _) eqn:?; [reflexivity|].
+    rewrite Nat.eqb_sym in Heqb; rewrite Heqb; reflexivity.
+  Qed.
+
+  Theorem lookup_empty : forall x,
+      lookup empty x = None.
+  Proof. reflexivity. Qed.
+End FunEnv.
