coq/theories/functional/FunProperties.v
@@ -1,0 +1,230 @@
+Require Import Coq.Lists.List.
+Require Import Coq.Strings.Ascii.
+Import ListNotations.
+Require Import impboot.functional.FunSyntax.
+Import Nat.
+Require Import impboot.utils.Llist.
+Require Import impboot.functional.FunSemantics.
+Require Import impboot.functional.FunValues.
+
+(* What do I induct on here? induction e just gives me IH for singleton lists *)
+(* Lemma Eval_deterministic_single : forall e s env a1 a2,
+  env |- ([e], s) ---> a1 ->
+  env |- ([e], s) ---> a2 ->
+  a1 = a2.
+Proof.
+  intros e s env a1 a2 H1 H2.
+  induction e; try reflexivity; destruct a1, a2; simpl in *; subst.
+  all: inversion H1; inversion H2; subst; eauto; try congruence.
+  - unfold eval_op in *.
+Admitted. *)
+
+(*
+TODO(kπ):
+- for proofs use pa explicit tuples, instread of one variable that is a tuple
+*)
+
+Lemma Eval_deterministic : forall e s env a1v a1s,
+  env |- (e, s) ---> (a1v, a1s) ->
+  forall a2v a2s,
+    env |- (e, s) ---> (a2v, a2s) ->
+    (a1v, a1s) = (a2v, a2s).
+Proof.
+  induction 1; inversion 1; simpl in *; subst; try congruence.
+  - apply IHeval1 in EVAL_HEAD; inversion EVAL_HEAD; subst.
+    apply IHeval2 in EVAL_TAIL; inversion EVAL_TAIL; subst.
+    reflexivity.
+  - apply IHeval in EVAL_ARGS. congruence.
+  - apply IHeval1 in EVAL_RHS; inversion EVAL_RHS; subst.
+    apply IHeval2 in EVAL_RES; inversion EVAL_RES; subst.
+    reflexivity.
+  - apply IHeval1 in EVAL_COND; inversion EVAL_COND; subst.
+    remember (take_branch test vs0 s4) as b1.
+    destruct b1; destruct r; inversion TAKE_BRANCH; inversion TAKE_BRANCH0; subst.
+    apply IHeval2 in EVAL_RES; inversion EVAL_RES; subst.
+    reflexivity.
+  - apply IHeval1 in EVAL_ARGS; inversion EVAL_ARGS; subst.
+    remember (env_and_body fname vs0 s4) as b1.
+    destruct b1; try destruct p; inversion ENV_BODY; inversion ENV_BODY0; subst.
+    apply IHeval2 in EVAL_BODY; inversion EVAL_BODY; subst.
+    reflexivity.
+Qed.
+
+Ltac cleanup :=
+  repeat match goal with
+  | [ H : context[fst ?x] |- _ ] => destruct x; simpl in *
+  | [ |- exists _, _ ] => eexists
+  | [ |- _ /\ _ ] => split
+  | [ H : _ /\ _ |- _ ] => destruct H
+  | [ H : exists _, _ |- _ ] => destruct H
+  | _ => intros
+  | _ => progress subst
+  | _ => progress eauto
+  | _ => progress simpl in *
+  | _ => constructor
+  | _ => congruence
+  end.
+
+Lemma Call_eq: forall fname xs s1 env a1v a1s,
+  env |- ([Call fname xs], s1) ---> (a1v, a1s) <->
+  exists vs s2 v s3,
+    env |- (xs, s1) ---> (vs, s2) /\
+    eval_app fname vs s2 (v, s3) /\ (a1v, a1s) = ([v],s3).
+Proof.
+  repeat split; intros; try inversion H; subst; try constructor.
+  all: repeat match goal with
+  | [ H : context[fst ?x] |- _ ] => destruct x; simpl in *
+  | [ |- exists _, _ ] => eexists
+  | [ |- _ /\ _ ] => split
+  | [ H : _ /\ _ |- _ ] => destruct H
+  | [ H : exists _, _ |- _ ] => destruct H
+  | _ => progress subst
+  | _ => progress eauto
+  | _ => progress simpl in *
+  | _ => constructor
+  | _ => congruence
+  end.
+  - eapply App_intro; eauto.
+  - inversion H2; inversion H3; inversion H1; subst.
+    eapply Eval_Call; eauto.
+Qed.
+
+Theorem Eval_eq :
+  (forall s env a1vs a1s, env |- ([], s) ---> (a1vs, a1s) <-> (a1vs, a1s) = ([], s)) /\
+  (forall y xs x s1 env a1vs a1s,
+     env |- (x :: y :: xs, s1) ---> (a1vs, a1s) <->
+     exists v vs s2 s3,
+       (a1vs, a1s) = (v::vs, s3) /\
+       (env |- ([x], s1) ---> ([v], s2)) /\
+       (env |- (y :: xs, s2) ---> (vs, s3))) /\
+  (forall v s env a1vs a1s, env |- ([Const v], s) ---> (a1vs, a1s) <-> (a1vs, a1s) = ([Num v], s)) /\
+  (forall s n env a1vs a1s,
+     env |- ([Var n], s) ---> (a1vs, a1s) <->
+     exists v, (a1vs, a1s) = ([v], s) /\ Env.lookup env n = Some v) /\
+  (forall xs s1 f env a1vs a1s,
+     env |- ([Op f xs], s1) ---> (a1vs, a1s) <->
+     exists vs s2 s3 v,
+       (a1vs, a1s) = ([v], s3) /\
+       env |- (xs, s1) ---> (vs, s2) /\
+       eval_op f vs s2 = (Res v, s3)) /\
+  (forall y x s1 n env a1vs a1s,
+     env |- ([Let n x y], s1) ---> (a1vs, a1s) <->
+     exists v1 s2 s3 v2,
+       (a1vs, a1s) = ([v2], s3) /\
+       env |- ([x], s1) ---> ([v1], s2) /\
+       (Env.insert (n, v1) env) |- ([y], s2) ---> ([v2], s3)) /\
+  (forall z y xs test s1 env a1vs a1s,
+     env |- ([If test xs y z], s1) ---> (a1vs, a1s) <->
+     exists vs s2 b v s3,
+       (a1vs, a1s) = ([v], s3) /\
+       env |- (xs, s1) ---> (vs, s2) /\
+       take_branch test vs s2 = (Res b, s2) /\
+       env |- ([if b then y else z], s2) ---> ([v], s3)) /\
+  (forall xs s1 fname env a1vs a1s,
+     env |- ([Call fname xs], s1) ---> (a1vs, a1s) <->
+     exists vs s2 v s3,
+       env |- (xs, s1) ---> (vs, s2) /\
+       eval_app fname vs s2 (v, s3) /\
+       (a1vs, a1s) = ([v], s3)).
+Proof.
+  repeat split; intros; try inversion H; subst; try constructor.
+  all: repeat match goal with
+  | [ H : context[fst ?x] |- _ ] => destruct x; simpl in *
+  | [ |- exists _, _ ] => eexists
+  | [ |- _ /\ _ ] => split
+  | [ H : _ /\ _ |- _ ] => destruct H
+  | [ H : exists _, _ |- _ ] => destruct H
+  | [ H : (_, _) = _ |- _ ] => inversion H; subst
+  | _ => progress subst
+  | _ => progress eauto
+  | _ => progress simpl in *
+  | _ => constructor
+  | _ => congruence
+  end.
+  - eapply Eval_Cons; eauto.
+  - rewrite H1 in H2; inversion H2; subst.
+    eapply Eval_Var; eauto.
+  - eapply Eval_Op; inversion H0; eauto.
+  - eapply Eval_Let; inversion H0; eauto.
+  - eapply Eval_If; inversion H0; eauto.
+  - eapply App_intro; eauto.
+  - inversion H2; subst.
+    eapply (Call_eq fname xs s1 env [x1] x2).
+    eexists x, x0, x1, x2; eauto.
+Qed.
+
+Lemma Eval_eq_Nil : forall s env a1v a1s, env |- ([], s) ---> (a1v, a1s) <-> (a1v, a1s) = ([], s).
+Proof.
+  destruct Eval_eq; eauto.
+Qed.
+
+Lemma Eval_eq_Cons : forall y xs x s1 env a1v a1s,
+  env |- (x :: y :: xs, s1) ---> (a1v, a1s) <->
+  exists v vs s2 s3,
+    (a1v, a1s) = (v::vs, s3) /\
+    (env |- ([x], s1) ---> ([v], s2)) /\
+    (env |- (y :: xs, s2) ---> (vs, s3)).
+Proof.
+  destruct Eval_eq; cleanup.
+  eapply H0; eauto.
+Qed.
+
+Lemma Eval_eq_Const : forall v s env a1v a1s,
+  env |- ([Const v], s) ---> (a1v, a1s) <-> (a1v, a1s) = ([Num v], s).
+Proof.
+  destruct Eval_eq; cleanup.
+  eapply H1; eauto.
+Qed.
+
+Lemma Eval_eq_Var : forall s n env a1v a1s,
+  env |- ([Var n], s) ---> (a1v, a1s) <->
+  exists v, (a1v, a1s) = ([v], s) /\ Env.lookup env n = Some v.
+Proof.
+  destruct Eval_eq; cleanup.
+  eapply H2; eauto.
+Qed.
+
+Lemma Eval_eq_Op : forall xs s1 f env a1v a1s,
+  env |- ([Op f xs], s1) ---> (a1v, a1s) <->
+  exists vs s2 s3 v,
+    (a1v, a1s) = ([v], s3) /\
+    env |- (xs, s1) ---> (vs, s2) /\
+    eval_op f vs s2 = (Res v, s3).
+Proof.
+  destruct Eval_eq; cleanup.
+  eapply H3; eauto.
+Qed.
+
+Lemma Eval_eq_Let : forall y x s1 n env a1v a1s,
+  env |- ([Let n x y], s1) ---> (a1v, a1s) <->
+  exists v1 s2 s3 v2,
+    (a1v, a1s) = ([v2], s3) /\
+    env |- ([x], s1) ---> ([v1], s2) /\
+    (Env.insert (n, v1) env) |- ([y], s2) ---> ([v2], s3).
+Proof.
+  destruct Eval_eq; cleanup.
+  eapply H4; eauto.
+Qed.
+
+Lemma Eval_eq_If : forall z y xs test s1 env a1v a1s,
+  env |- ([If test xs y z], s1) ---> (a1v, a1s) <->
+  exists vs s2 b v s3,
+    (a1v, a1s) = ([v], s3) /\
+    env |- (xs, s1) ---> (vs, s2) /\
+    take_branch test vs s2 = (Res b, s2) /\
+    env |- ([if b then y else z], s2) ---> ([v], s3).
+Proof.
+  destruct Eval_eq; cleanup.
+  eapply H5; eauto.
+Qed.
+
+Lemma Eval_eq_Call : forall xs s1 fname env a1v a1s,
+  env |- ([Call fname xs], s1) ---> (a1v, a1s) <->
+  exists vs s2 v s3,
+    env |- (xs, s1) ---> (vs, s2) /\
+    eval_app fname vs s2 (v, s3) /\
+    (a1v, a1s) = ([v], s3).
+Proof.
+  destruct Eval_eq; cleanup.
+  eapply H6; eauto.
+Qed.
