coq/theories/functional/FunSyntax.v
@@ -4,34 +4,108 @@ Import ListNotations.
 Notation name := nat.
 
 Inductive op : Type :=
-  | Add
-  | Sub
-  | Div
-  | Cons
-  | Head
-  | Tail
-  | Read
-  | Write.
+| Add
+| Sub
+| Div
+| Cons
+| Head
+| Tail
+| Read
+| Write.
 
 Inductive test : Type :=
-  | Less
-  | Equal.
+| Less
+| Equal.
 
 Inductive exp : Type :=
-  | Const (n : nat)                                (* constant number            *)
-  | Var (n : name)                                 (* local variable             *)
-  | Op (o : op) (args : list exp)                  (* primitive operations       *)
-  | If (t : test) (conds : list exp) (e1 e2 : exp) (* if test .. then .. else .. *)
-  | Let (n : name) (e1 e2 : exp)                   (* let name = .. in ..        *)
-  | Call (f : name) (args : list exp).             (* call a function            *)
+| Const (n : nat)                                (* constant number            *)
+| Var (n : name)                                 (* local variable             *)
+| Op (o : op) (args : list exp)                  (* primitive operations       *)
+| If (t : test) (conds : list exp) (e1 e2 : exp) (* if test .. then .. else .. *)
+| Let (n : name) (e1 e2 : exp)                   (* let name = .. in ..        *)
+| Call (f : name) (args : list exp).             (* call a function            *)
+
+Fixpoint exp_ind_str (P : exp -> Prop)
+  (HConst : forall n : nat, P (Const n))
+  (HVar : forall n : name, P (Var n))
+  (HOp : forall (o : op) (args : list exp), Forall P args -> P (Op o args))
+  (HIf : forall (t : test) (conds : list exp) (e1 e2 : exp),
+      Forall P conds -> P e1 -> P e2 -> P (If t conds e1 e2))
+  (HLet : forall (n : name) (e1 e2 : exp), P e1 -> P e2 -> P (Let n e1 e2))
+  (HCall : forall (f : name) (args : list exp), Forall P args -> P (Call f args))
+  (e : exp) : P e :=
+  match e as e0 return P e0 with
+  | Const n =>
+    HConst n
+  | Var n =>
+    HVar n
+  | Op o args =>
+    HOp o args ((fix list_exp_ind (l : list exp) : Forall P l :=
+                  match l with
+                  | [] => Forall_nil P
+                  | e :: l' => Forall_cons e (exp_ind_str P HConst HVar HOp HIf HLet HCall e)
+                                      (list_exp_ind l')
+                  end) args)
+  | If t conds e1 e2 =>
+    HIf t conds e1 e2 ((fix list_exp_ind (l : list exp) : Forall P l :=
+                          match l with
+                          | [] => Forall_nil P
+                          | e :: l' => Forall_cons e (exp_ind_str P HConst HVar HOp HIf HLet HCall e)
+                                                (list_exp_ind l')
+                          end) conds) (exp_ind_str P HConst HVar HOp HIf HLet HCall e1)
+                          (exp_ind_str P HConst HVar HOp HIf HLet HCall e2)
+  | Let n e1 e2 =>
+    HLet n e1 e2 (exp_ind_str P HConst HVar HOp HIf HLet HCall e1)
+                 (exp_ind_str P HConst HVar HOp HIf HLet HCall e2)
+  | Call f args =>
+    HCall f args ((fix list_exp_ind (l : list exp) : Forall P l :=
+                    match l with
+                    | [] => Forall_nil P
+                    | e :: l' => Forall_cons e (exp_ind_str P HConst HVar HOp HIf HLet HCall e)
+                                          (list_exp_ind l')
+                    end) args)
+  end.
+
+(* Not decreasing *)
+Fail Fixpoint exp_ind_list (P : list exp -> Prop)
+  (HNil : P [])
+  (HCons : forall e es, P [e] -> P es -> P (e :: es))
+  (HConst : forall n : nat, P [Const n])
+  (HVar : forall n : name, P [Var n])
+  (HOp : forall (o : op) (args : list exp), P args -> P [Op o args])
+  (HIf : forall (t : test) (conds : list exp) (e1 e2 : exp),
+      P conds -> P [e1] -> P [e2] -> P [If t conds e1 e2])
+  (HLet : forall (n : name) (e1 e2 : exp), P [e1] -> P [e2] -> P [Let n e1 e2])
+  (HCall : forall (f : name) (args : list exp), P args -> P [Call f args])
+  (es : list exp) : P es :=
+  match es with
+  | [] => HNil
+  | [Const n] => HConst n
+  | [Var n] => HVar n
+  | [Op o args] =>
+    HOp o args (exp_ind_list P HNil HCons HConst HVar HOp HIf HLet HCall args)
+  | [If t conds e1 e2] =>
+    HIf t conds e1 e2 (exp_ind_list P HNil HCons HConst HVar HOp HIf HLet HCall conds)
+                      (exp_ind_list P HNil HCons HConst HVar HOp HIf HLet HCall [e1])
+                      (exp_ind_list P HNil HCons HConst HVar HOp HIf HLet HCall [e2])
+  | [Let n e1 e2] =>
+    HLet n e1 e2 (exp_ind_list P HNil HCons HConst HVar HOp HIf HLet HCall [e1])
+                 (exp_ind_list P HNil HCons HConst HVar HOp HIf HLet HCall [e2])
+  | [Call f args] =>
+    HCall f args (exp_ind_list P HNil HCons HConst HVar HOp HIf HLet HCall args)
+  | e :: es' =>
+    HCons e es'
+           (exp_ind_list P HNil HCons HConst HVar HOp HIf HLet HCall [e])
+           (exp_ind_list P HNil HCons HConst HVar HOp HIf HLet HCall es')
+  end.
 
 Inductive dec : Type :=
-  | Defun (n : name) (params : list name) (body : exp). (* func name, formal params, body *)
+| Defun (n : name) (params : list name) (body : exp). (* func name, formal params, body *)
 
 (* a complete program is a list of function declarations followed by *)
 (* an expression to evaluate *)
 Inductive prog : Type :=
-  | Program (defs : list dec) (main : exp).
+| Program (defs : list dec) (main : exp).
 
 Definition get_main (p : prog) : exp :=
   match p with
