coq/theories/functional/FunValues.v
@@ -1,0 +1,112 @@
+Require Import Coq.Lists.List.
+Require Import Coq.Strings.Ascii.
+Require Import Coq.Arith.PeanoNat.
+Require Import impboot.functional.FunSyntax.
+Import ListNotations.
+
+Notation name := nat.
+
+Inductive Value :=
+  | Pair (v1 v2 : Value)
+  | Num (n : nat).
+
+Definition value_name (s : list ascii) : nat :=
+  fold_right (fun c acc => (nat_of_ascii c) * 256 + acc) 0 s.
+
+Definition value_list (xs : list Value) : Value :=
+  fold_right (fun x acc => Pair x acc) (Num 0) xs.
+
+Definition value_less (v1 v2 : Value) : bool :=
+  match v1, v2 with
+  | Num n1, Num n2 => n1 <? n2
+  | _, _ => false
+  end.
+
+Definition value_plus (v1 v2 : Value) : Value :=
+  match v1, v2 with
+  | Num n1, Num n2 => Num (n1 + n2)
+  | _, _ => Num 0
+  end.
+
+Definition value_minus (v1 v2 : Value) : Value :=
+  match v1, v2 with
+  | Num n1, Num n2 => Num (n1 - n2)
+  | _, _ => Num 0
+  end.
+
+Definition value_div (v1 v2 : Value) : Value :=
+  match v1, v2 with
+  | Num n1, Num n2 => if n2 =? 0 then Num 0 else Num (n1 / n2)
+  | _, _ => Num 0
+  end.
+
+Definition value_head (v : Value) : Value :=
+  match v with
+  | Pair x _ => x
+  | _ => v
+  end.
+
+Definition value_tail (v : Value) : Value :=
+  match v with
+  | Pair _ y => y
+  | _ => v
+  end.
+
+Definition value_cons (x y : Value) : Value :=
+  Pair x y.
+
+Definition value_bool (b : bool) : Value :=
+  if b then Num 1 else Num 0.
+
+Definition value_map (f : Value -> Value) (xs : list Value) : Value :=
+  value_list (List.map f xs).
+
+Definition value_pair (f g : Value -> Value) (p : Value * Value) : Value :=
+  match p with
+  | (x, y) => Pair (f x) (g y)
+  end.
+
+Definition value_option (f : Value -> Value) (o : option Value) : Value :=
+  match o with
+  | None => value_list []
+  | Some x => value_list [f x]
+  end.
+
+Definition value_char (c : ascii) : Value :=
+  Num (nat_of_ascii c).
+
+Definition value_isNum (v : Value) : bool :=
+  match v with
+  | Num _ => true
+  | _ => false
+  end.
+
+Definition value_getNum (v : Value) : nat :=
+  match v with
+  | Num n => n
+  | _ => 0
+  end.
+
+Definition value_el1 (v : Value) : Value :=
+  value_head (value_tail v).
+
+Definition value_el2 (v : Value) : Value :=
+  value_el1 (value_tail v).
+
+Definition value_el3 (v : Value) : Value :=
+  value_el2 (value_tail v).
+
+Theorem isNum_bool : forall b,
+  value_isNum (value_bool b) = true.
+Proof.
+  intros. destruct b; reflexivity.
+Qed.
+
+(* TODO(kπ) again problem with termination of this almost exact function *)
+Fail Fixpoint value_is_upper (n : nat) : bool :=
+  if n <? 256 then
+    if n <? 65 then false else
+    if n <? 91 then true else false
+  else value_is_upper (n / 256).
+
+Definition value_otherwise {A: Type} (x : A) : A := x.
